Progress on CallEx + Dispatcher refactoring.

example/CallEx.thy
@@ -33,38 +33,31 @@ contract A {
     }
 
 }
-squires $ ./solc  call.sol --overwrite --bin -o res 
-squires $ for f in res/*.bin ; do cat $f ; echo ; done
-608060405234801561001057600080fd5b506040516020806101f383398101806040528101908080519060200190929190505050806000806101000a81548173ffffffffffffffffffffffffffffffffffffffff021916908373ffffffffffffffffffffffffffffffffffffffff1602179055506000600181905550506101688061008b6000396000f300608060405260043610610041576000357c0100000000000000000000000000000000000000000000000000000000900463ffffffff16806344fd4fa014610046575b600080fd5b34801561005257600080fd5b5061005b610071565b6040518082815260200191505060405180910390f35b60008060009054906101000a900473ffffffffffffffffffffffffffffffffffffffff1673ffffffffffffffffffffffffffffffffffffffff166326121ff06040518163ffffffff167c0100000000000000000000000000000000000000000000000000000000028152600401602060405180830381600087803b1580156100f857600080fd5b505af115801561010c573d6000803e3d6000fd5b505050506040513d602081101561012257600080fd5b8101908080519060200190929190505050600181905550905600a165627a7a72305820b098d684bc2516a3af5106f6efd38d926edb67ea42c065bd94a63e7e988f19980029
-6080604052348015600f57600080fd5b5060a18061001e6000396000f300608060405260043610603f576000357c0100000000000000000000000000000000000000000000000000000000900463ffffffff16806326121ff0146044575b600080fd5b348015604f57600080fd5b506056606c565b6040518082815260200191505060405180910390f35b6000602a9050905600a165627a7a7230582056366c316c8eb1c2cb71b875b90a5eaf72d3069879bea637993dcf928cfb1cde0029
+squires $ ./solc  call.sol --overwrite --bin-runtime -o res
+squires $ for f in res/*.bin-runtime ; do cat $f ; echo ; done
+608060405260043610610041576000357c0100000000000000000000000000000000000000000000000000000000900463ffffffff16806344fd4fa014610046575b600080fd5b34801561005257600080fd5b5061005b610071565b6040518082815260200191505060405180910390f35b60008060009054906101000a900473ffffffffffffffffffffffffffffffffffffffff1673ffffffffffffffffffffffffffffffffffffffff166326121ff06040518163ffffffff167c0100000000000000000000000000000000000000000000000000000000028152600401602060405180830381600087803b1580156100f857600080fd5b505af115801561010c573d6000803e3d6000fd5b505050506040513d602081101561012257600080fd5b8101908080519060200190929190505050600181905550905600a165627a7a72305820b098d684bc2516a3af5106f6efd38d926edb67ea42c065bd94a63e7e988f19980029
+608060405260043610603f576000357c0100000000000000000000000000000000000000000000000000000000900463ffffffff16806326121ff0146044575b600080fd5b348015604f57600080fd5b506056606c565b6040518082815260200191505060405180910390f35b6000602a9050905600a165627a7a7230582056366c316c8eb1c2cb71b875b90a5eaf72d3069879bea637993dcf928cfb1cde0029
+s
+
 \<close>
 
 definition A_addr :: "address" where
  "A_addr \<equiv> 0x42"
 definition A_bytestr :: "byte list" where
- "A_bytestr \<equiv> bytes_of_hex_content ''608060405234801561001057600080fd5b506040516020806101f383398101806040528101908080519060200190929190505050806000806101000a81548173ffffffffffffffffffffffffffffffffffffffff021916908373ffffffffffffffffffffffffffffffffffffffff1602179055506000600181905550506101688061008b6000396000f300608060405260043610610041576000357c0100000000000000000000000000000000000000000000000000000000900463ffffffff16806344fd4fa014610046575b600080fd5b34801561005257600080fd5b5061005b610071565b6040518082815260200191505060405180910390f35b60008060009054906101000a900473ffffffffffffffffffffffffffffffffffffffff1673ffffffffffffffffffffffffffffffffffffffff166326121ff06040518163ffffffff167c0100000000000000000000000000000000000000000000000000000000028152600401602060405180830381600087803b1580156100f857600080fd5b505af115801561010c573d6000803e3d6000fd5b505050506040513d602081101561012257600080fd5b8101908080519060200190929190505050600181905550905600a165627a7a72305820b098d684bc2516a3af5106f6efd38d926edb67ea42c065bd94a63e7e988f19980029''"
+ "A_bytestr \<equiv> bytes_of_hex_content ''608060405260043610610041576000357c0100000000000000000000000000000000000000000000000000000000900463ffffffff16806344fd4fa014610046575b600080fd5b34801561005257600080fd5b5061005b610071565b6040518082815260200191505060405180910390f35b60008060009054906101000a900473ffffffffffffffffffffffffffffffffffffffff1673ffffffffffffffffffffffffffffffffffffffff166326121ff06040518163ffffffff167c0100000000000000000000000000000000000000000000000000000000028152600401602060405180830381600087803b1580156100f857600080fd5b505af115801561010c573d6000803e3d6000fd5b505050506040513d602081101561012257600080fd5b8101908080519060200190929190505050600181905550905600a165627a7a72305820b098d684bc2516a3af5106f6efd38d926edb67ea42c065bd94a63e7e988f19980029''"
 
 definition B_addr :: "address" where
  "B_addr \<equiv> 0x43"
 definition B_bytestr :: "byte list" where
- "B_bytestr \<equiv> bytes_of_hex_content ''6080604052348015600f57600080fd5b5060a18061001e6000396000f300608060405260043610603f576000357c0100000000000000000000000000000000000000000000000000000000900463ffffffff16806326121ff0146044575b600080fd5b348015604f57600080fd5b506056606c565b6040518082815260200191505060405180910390f35b6000602a9050905600a165627a7a7230582056366c316c8eb1c2cb71b875b90a5eaf72d3069879bea637993dcf928cfb1cde0029''"
+ "B_bytestr \<equiv> bytes_of_hex_content ''608060405260043610603f576000357c0100000000000000000000000000000000000000000000000000000000900463ffffffff16806326121ff0146044575b600080fd5b348015604f57600080fd5b506056606c565b6040518082815260200191505060405180910390f35b6000602a9050905600a165627a7a7230582056366c316c8eb1c2cb71b875b90a5eaf72d3069879bea637993dcf928cfb1cde0029
+s''"
 
 
 value "parse_bytes A_bytestr"
 
 definition
- "A_insts \<equiv> [Stack (PUSH_N [0x80]), Stack (PUSH_N [0x40]), Memory MSTORE, Info CALLVALUE, Dup 0, Arith ISZERO, Stack (PUSH_N [0, 0x10]), Pc JUMPI,
-  Stack (PUSH_N [0]), Dup 0, Unknown 0xFD, Pc JUMPDEST, Stack POP, Stack (PUSH_N [0x40]), Memory MLOAD, Stack (PUSH_N [0x20]), Dup 0,
-  Stack (PUSH_N [1, 0xF3]), Dup 3, Memory CODECOPY, Dup 1, Arith ADD, Dup 0, Stack (PUSH_N [0x40]), Memory MSTORE, Dup 1, Arith ADD,
-  Swap 0, Dup 0, Dup 0, Memory MLOAD, Swap 0, Stack (PUSH_N [0x20]), Arith ADD, Swap 0, Swap 2, Swap 1, Swap 0, Stack POP, Stack POP,
-  Stack POP, Dup 0, Stack (PUSH_N [0]), Dup 0, Stack (PUSH_N [1, 0]), Arith EXP, Dup 1, Storage SLOAD, Dup 1,
-  Stack (PUSH_N [0xFF, 0xFF, 0xFF, 0xFF, 0xFF, 0xFF, 0xFF, 0xFF, 0xFF, 0xFF, 0xFF, 0xFF, 0xFF, 0xFF, 0xFF, 0xFF, 0xFF, 0xFF, 0xFF, 0xFF]),
-  Arith MUL, Bits inst_NOT, Bits inst_AND, Swap 0, Dup 3,
-  Stack (PUSH_N [0xFF, 0xFF, 0xFF, 0xFF, 0xFF, 0xFF, 0xFF, 0xFF, 0xFF, 0xFF, 0xFF, 0xFF, 0xFF, 0xFF, 0xFF, 0xFF, 0xFF, 0xFF, 0xFF, 0xFF]),
-  Bits inst_AND, Arith MUL, Bits inst_OR, Swap 0, Storage SSTORE, Stack POP, Stack (PUSH_N [0]), Stack (PUSH_N [1]), Dup 1, Swap 0,
-  Storage SSTORE, Stack POP, Stack POP, Stack (PUSH_N [1, 0x68]), Dup 0, Stack (PUSH_N [0, 0x8B]), Stack (PUSH_N [0]), Memory CODECOPY,
-  Stack (PUSH_N [0]), Misc RETURN, Misc STOP, Stack (PUSH_N [0x80]), Stack (PUSH_N [0x40]), Memory MSTORE, Stack (PUSH_N [4]),
-  Info CALLDATASIZE, Arith inst_LT, Stack (PUSH_N [0, 0x41]), Pc JUMPI, Stack (PUSH_N [0]), Stack CALLDATALOAD,
+ "A_insts \<equiv> [Stack (PUSH_N [0x80]), Stack (PUSH_N [0x40]), Memory MSTORE, Stack (PUSH_N [4]), Info CALLDATASIZE, Arith inst_LT,
+  Stack (PUSH_N [0, 0x41]), Pc JUMPI, Stack (PUSH_N [0]), Stack CALLDATALOAD,
   Stack (PUSH_N [1, 0, 0, 0, 0, 0, 0, 0, 0, 0, 0, 0, 0, 0, 0, 0, 0, 0, 0, 0, 0, 0, 0, 0, 0, 0, 0, 0, 0]), Swap 0, Arith DIV,
   Stack (PUSH_N [0xFF, 0xFF, 0xFF, 0xFF]), Bits inst_AND, Dup 0, Stack (PUSH_N [0x44, 0xFD, 0x4F, 0xA0]), Arith inst_EQ,
   Stack (PUSH_N [0, 0x46]), Pc JUMPI, Pc JUMPDEST, Stack (PUSH_N [0]), Dup 0, Unknown 0xFD, Pc JUMPDEST, Info CALLVALUE, Dup 0,
@@ -94,7 +87,7 @@ definition
 
 definition
   bytestr_to_program :: "byte list \<Rightarrow> program" where
- "bytestr_to_program bytestr \<equiv> program_of_lst (parse_bytes bytestr)
+ "bytestr_to_program bstr \<equiv> program_of_lst (parse_bytes bstr)
                                               (\<lambda>xs i. if i < length xs then Some (xs ! nat i) else None)"
 
 definition
@@ -103,8 +96,10 @@ definition
 
 definition transaction_nonce :: w256 where
  "transaction_nonce \<equiv> 0x13"
+
 definition
  "acc_bal = 0x1000000000000"
+
 definition accounts :: "address \<Rightarrow> block_account"  where
  "accounts \<equiv> undefined(
     A_addr := \<lparr>   block_account_address = A_addr, 
@@ -134,6 +129,7 @@ term global_sem
 
 definition
  "tr_gas_limit' \<equiv> 0x1000000"
+
 definition tr :: transaction where
  "tr \<equiv> \<lparr> tr_from = user, tr_to = Some A_addr, tr_gas_limit = tr_gas_limit', tr_gas_price= 100, tr_value = 0, tr_nonce = transaction_nonce, tr_data = [] \<rparr>"
 
@@ -272,18 +268,93 @@ lemma bytes_of_hex_content_not_Nil:
   apply (rename_tac ys, case_tac ys; clarsimp)
   done
 
-definition bytestr :: "'a::len0 word \<Rightarrow> byte list"  where
- "bytestr \<equiv> word_rsplit"
 
-abbreviation "blk_num \<equiv> block_number_pred"
+definition "blocks_A_insts \<equiv> build_blocks A_insts"
+value "blocks_A_insts"
+lemma blocks_A_insts_simp:
+ "blocks_A_insts = [(0, [(0, Stack (PUSH_N [0x80])), (2, Stack (PUSH_N [0x40])), (4, Memory MSTORE), (5, Stack (PUSH_N [4])), (7, Info CALLDATASIZE),
+       (8, Arith inst_LT), (9, Stack (PUSH_N [0, 0x41]))],
+   Jumpi),
+  (13,
+   [(13, Stack (PUSH_N [0])), (15, Stack CALLDATALOAD),
+    (16, Stack (PUSH_N [1, 0, 0, 0, 0, 0, 0, 0, 0, 0, 0, 0, 0, 0, 0, 0, 0, 0, 0, 0, 0, 0, 0, 0, 0, 0, 0, 0, 0])), (46, Swap 0),
+    (47, Arith DIV), (48, Stack (PUSH_N [0xFF, 0xFF, 0xFF, 0xFF])), (53, Bits inst_AND), (54, Dup 0),
+    (55, Stack (PUSH_N [0x44, 0xFD, 0x4F, 0xA0])), (60, Arith inst_EQ), (61, Stack (PUSH_N [0, 0x46]))],
+   Jumpi),
+  (65, [(65, Pc JUMPDEST), (66, Stack (PUSH_N [0])), (68, Dup 0), (69, Unknown 0xFD)], Terminal),
+  (70, [(70, Pc JUMPDEST), (71, Info CALLVALUE), (72, Dup 0), (73, Arith ISZERO), (74, Stack (PUSH_N [0, 0x52]))], Jumpi),
+  (78, [(78, Stack (PUSH_N [0])), (80, Dup 0), (81, Unknown 0xFD)], Terminal),
+  (82, [(82, Pc JUMPDEST), (83, Stack POP), (84, Stack (PUSH_N [0, 0x5B])), (87, Stack (PUSH_N [0, 0x71]))], Jump),
+  (91,
+   [(91, Pc JUMPDEST), (92, Stack (PUSH_N [0x40])), (94, Memory MLOAD), (95, Dup 0), (96, Dup 2), (97, Dup 1), (98, Memory MSTORE),
+    (99, Stack (PUSH_N [0x20])), (101, Arith ADD), (102, Swap 1), (103, Stack POP), (104, Stack POP), (105, Stack (PUSH_N [0x40])),
+    (107, Memory MLOAD), (108, Dup 0), (109, Swap 1), (110, Arith SUB), (111, Swap 0), (112, Misc RETURN)],
+   Terminal),
+  (113,
+   [(113, Pc JUMPDEST), (114, Stack (PUSH_N [0])), (116, Dup 0), (117, Stack (PUSH_N [0])), (119, Swap 0), (120, Storage SLOAD),
+    (121, Swap 0), (122, Stack (PUSH_N [1, 0])), (125, Arith EXP), (126, Swap 0), (127, Arith DIV),
+    (128,
+     Stack
+      (PUSH_N [0xFF, 0xFF, 0xFF, 0xFF, 0xFF, 0xFF, 0xFF, 0xFF, 0xFF, 0xFF, 0xFF, 0xFF, 0xFF, 0xFF, 0xFF, 0xFF, 0xFF, 0xFF, 0xFF, 0xFF])),
+    (149, Bits inst_AND),
+    (150,
+     Stack
+      (PUSH_N [0xFF, 0xFF, 0xFF, 0xFF, 0xFF, 0xFF, 0xFF, 0xFF, 0xFF, 0xFF, 0xFF, 0xFF, 0xFF, 0xFF, 0xFF, 0xFF, 0xFF, 0xFF, 0xFF, 0xFF])),
+    (171, Bits inst_AND), (172, Stack (PUSH_N [0x26, 0x12, 0x1F, 0xF0])), (177, Stack (PUSH_N [0x40])), (179, Memory MLOAD), (180, Dup 1),
+    (181, Stack (PUSH_N [0xFF, 0xFF, 0xFF, 0xFF])), (186, Bits inst_AND),
+    (187, Stack (PUSH_N [1, 0, 0, 0, 0, 0, 0, 0, 0, 0, 0, 0, 0, 0, 0, 0, 0, 0, 0, 0, 0, 0, 0, 0, 0, 0, 0, 0, 0])), (217, Arith MUL),
+    (218, Dup 1), (219, Memory MSTORE), (220, Stack (PUSH_N [4])), (222, Arith ADD), (223, Stack (PUSH_N [0x20])),
+    (225, Stack (PUSH_N [0x40])), (227, Memory MLOAD), (228, Dup 0), (229, Dup 3), (230, Arith SUB), (231, Dup 1),
+    (232, Stack (PUSH_N [0])), (234, Dup 7), (235, Dup 0), (236, Info EXTCODESIZE), (237, Arith ISZERO), (238, Dup 0), (239, Arith ISZERO),
+    (240, Stack (PUSH_N [0, 0xF8]))],
+   Jumpi),
+  (244, [(244, Stack (PUSH_N [0])), (246, Dup 0), (247, Unknown 0xFD)], Terminal),
+  (248, [(248, Pc JUMPDEST), (249, Stack POP), (250, Info GAS), (251, Misc CALL)], Terminal),
+  (252, [(252, Arith ISZERO), (253, Dup 0), (254, Arith ISZERO), (255, Stack (PUSH_N [1, 0xC]))], Jumpi),
+  (259, [(259, Unknown 0x3D)], Terminal), (260, [(260, Stack (PUSH_N [0])), (262, Dup 0), (263, Unknown 0x3E)], Terminal),
+  (264, [(264, Unknown 0x3D)], Terminal), (265, [(265, Stack (PUSH_N [0])), (267, Unknown 0xFD)], Terminal),
+  (268,
+   [(268, Pc JUMPDEST), (269, Stack POP), (270, Stack POP), (271, Stack POP), (272, Stack POP), (273, Stack (PUSH_N [0x40])),
+    (275, Memory MLOAD), (276, Unknown 0x3D)],
+   Terminal),
+  (277, [(277, Stack (PUSH_N [0x20])), (279, Dup 1), (280, Arith inst_LT), (281, Arith ISZERO), (282, Stack (PUSH_N [1, 0x22]))], Jumpi),
+  (286, [(286, Stack (PUSH_N [0])), (288, Dup 0), (289, Unknown 0xFD)], Terminal),
+  (290,
+   [(290, Pc JUMPDEST), (291, Dup 1), (292, Arith ADD), (293, Swap 0), (294, Dup 0), (295, Dup 0), (296, Memory MLOAD), (297, Swap 0),
+    (298, Stack (PUSH_N [0x20])), (300, Arith ADD), (301, Swap 0), (302, Swap 2), (303, Swap 1), (304, Swap 0), (305, Stack POP),
+    (306, Stack POP), (307, Stack POP), (308, Stack (PUSH_N [1])), (310, Dup 1), (311, Swap 0), (312, Storage SSTORE), (313, Stack POP),
+    (314, Swap 0)],
+   Jump),
+  (316, [(316, Misc STOP)], Terminal),
+  (317, [(317, Log LOG1), (318, Stack (PUSH_N [0x62, 0x7A, 0x7A, 0x72, 0x30, 0x58])), (325, Arith SHA3), (326, Unknown 0xB0)], Terminal),
+  (327, [(327, Swap 8), (328, Unknown 0xD6)], Terminal), (329, [(329, Dup 4), (330, Unknown 0xBC)], Terminal),
+  (331, [(331, Unknown 0x25)], Terminal), (332, [(332, Bits inst_AND), (333, Log LOG3), (334, Unknown 0xAF)], Terminal),
+  (335, [(335, Memory MLOAD), (336, Arith MOD), (337, Unknown 0xF6)], Terminal), (338, [(338, Unknown 0xEF)], Terminal),
+  (339, [(339, Unknown 0xD3)], Terminal),
+  (340,
+   [(340, Dup 0xD), (341, Swap 2),
+    (342, Stack (PUSH_N [0xDB, 0x67, 0xEA, 0x42, 0xC0, 0x65, 0xBD, 0x94, 0xA6, 0x3E, 0x7E, 0x98, 0x8F, 0x19, 0x98])), (358, Misc STOP)],
+   Terminal),
+  (359, [(359, Unknown 0x29)], Terminal)]"
+  by eval
 
-definition
-  bytestr_to_w256 :: "byte list \<Rightarrow> w256"  where
- "bytestr_to_w256 \<equiv> word_rcat"
-
+definition A_hash :: "32 word" where
+ "A_hash \<equiv> 0x44fd4fa0"
 
 lemma
- "bbtriple net
+  bit_mask_rev[simp]
+  address_mask_ucast[simp] address_mask_ucast[simplified word_bool_alg.conj.commute, simp]
+  ucast_and_w256_drop[simp]
+  transfer_hash_def[simp]
+  word_bool_alg.conj.commute[simp]
+  length_word_rsplit_4[simp]
+  ucast_160_upto_256_eq[simp]
+  hash_diff[simp]
+  eval_bit_mask[simp]
+len_bytestr_simps[simp]
+shows
+
+ "\<exists>Q. bbtriple net
  ( program_counter 0 ** stack_height 0 **
    sent_data (bytestr A_hash) **
    sent_value 0 ** caller sender ** blk_num bn **
@@ -298,7 +369,106 @@ lemma
    memory (0x60::w256) (bytestr_to_w256 [y]) **
    log_number log_num **
    this_account this)
- (build_blocks A_insts) Q"
+ (blocks_A_insts) (action (ContractCall args) ** Q)"
+  including dispatcher_bundle
+  apply (rule exI)
+  apply (simp add: blocks_A_insts_simp)
+  apply (simp add: bbtriple_def )
+  apply (block_vcg; (solves \<open>clarsimp\<close>)?)
+   apply (block_vcg)
+  apply (simp add: bytestr_def length_word_rsplit_32)
+   apply (simp add: A_hash_def)
+  apply (block_vcg)
+
+   apply (block_vcg)
+
+    apply split_conds
+  apply (simp add: A_hash_def bytestr_def)
+    apply (block_vcg)
+
+
+  apply (blocks_rule_vcg; (rule refl)?)
+      apply triple_seq_vcg
+             apply clarsimp
+             apply order_sep_conj
+  apply (sep_cancel)
+             apply (sep_cancel)
+
+             apply clarsimp
+             apply (sep_cancel)
+             apply (simp add: Gverylow_def pure_def)
+             apply order_sep_conj
+  apply (sep_cancel)
+             apply (sep_cancel)
+             apply (simp add: Gverylow_def pure_def)
+  apply (sep_imp_solve simp: Gverylow_def)
+             apply order_sep_conj
+  apply (sep_cancel)
+             apply order_sep_conj
+  apply (sep_cancel)
+             apply order_sep_conj
+  apply (sep_cancel)
+             apply order_sep_conj
+  apply (sep_cancel)
+             apply order_sep_conj
+           apply (sep_cancel)
+  apply (simp add: word_rcat_simps)
+             apply (order_sep_conj, sep_cancel)
+             apply (order_sep_conj, sep_cancel)
+           apply (order_sep_conj, sep_cancel)
+  find_theorems length word_rsplit 32
+           apply (clarsimp simp: Gverylow_def length_word_rsplit_32 Cmem_def gas_simps Gmemory_def M_def)
+  apply assumption
+             apply (order_sep_conj, sep_cancel)
+             apply (order_sep_conj, sep_cancel)
+           apply (clarsimp simp: Gverylow_def length_word_rsplit_32 Cmem_def gas_simps Gmemory_def M_def word_rcat_simps)
+  apply sep_cancel
+  apply sep_cancel
+          apply sep_cancel
+           apply (clarsimp simp: Gverylow_def length_word_rsplit_32 Cmem_def gas_simps Gmemory_def M_def)
+             apply (order_sep_conj, sep_cancel)
+             apply (order_sep_conj, sep_cancel)
+             apply (order_sep_conj, sep_cancel)
+           apply (clarsimp simp: Gverylow_def length_word_rsplit_32 Cmem_def gas_simps Gmemory_def M_def word_rcat_simps)
+          apply sep_cancel
+             apply (order_sep_conj, sep_cancel)
+             apply (order_sep_conj, sep_cancel)
+           apply (clarsimp simp: Gverylow_def length_word_rsplit_32 Cmem_def gas_simps Gmemory_def M_def word_rcat_simps)
+             apply (order_sep_conj, sep_cancel)
+             apply (order_sep_conj, sep_cancel)
+             apply (order_sep_conj, sep_cancel)
+           apply (clarsimp simp: Gverylow_def length_word_rsplit_32 Cmem_def gas_simps Gmemory_def M_def word_rcat_simps)
+             apply (order_sep_conj, sep_cancel)
+             apply (order_sep_conj, sep_cancel)
+           apply (clarsimp simp: Gverylow_def length_word_rsplit_32 Cmem_def gas_simps Gmemory_def M_def word_rcat_simps)
+             apply (order_sep_conj, sep_cancel)
+             apply (order_sep_conj, sep_cancel)
+           apply (clarsimp simp: Gverylow_def length_word_rsplit_32 Cmem_def gas_simps Gmemory_def M_def word_rcat_simps)
+             apply (order_sep_conj, sep_cancel)
+             apply (order_sep_conj, sep_cancel)
+             apply (order_sep_conj, sep_cancel)
+             apply (order_sep_conj, sep_cancel)
+             apply (order_sep_conj, sep_cancel)
+             apply (order_sep_conj, sep_cancel)
+           apply (clarsimp simp: Gverylow_def length_word_rsplit_32 Cmem_def gas_simps Gmemory_def M_def word_rcat_simps inst_size_def)
+      apply (order_sep_conj, sep_cancel)
+  apply simp
+    apply (clarsimp simp: Gverylow_def length_word_rsplit_32 Cmem_def gas_simps Gmemory_def M_def word_rcat_simps inst_size_def)
+  apply (rule conjI, rule refl, rule refl)
+(*   apply triple_blocks_vcg
+  apply (block_vcg)
+ *)  apply split_conds
+  apply (blocks_rule_vcg; (rule refl)?)
+      apply triple_seq_vcg
+             apply clarsimp
+             apply order_sep_conj
+  apply (sep_cancel)
+             apply (sep_cancel)
+
+
+          apply (sep_imp_solve2)
+  apply (sep_imp_solve2)
+
   oops
 
 lemma A_calls_B_spec:
